extraction: Give telescopes a dependent type
This makes working with Fiat-level bindings nicer, and yields a nicer
framework to talk about ADTs. There are still a few admits here and
there however.

src/CertifiedExtraction/CompUtils.v
@@ -7,43 +7,34 @@ Require Import
         Bedrock.Memory
         Bedrock.Platform.Facade.DFacade.
 
-Class FacadeWrapper (WrappingType WrappedType: Type) :=
-  { wrap:        WrappedType -> WrappingType;
-    unwrap:      WrappingType -> option WrappedType;
-    wrap_unwrap: forall v, unwrap (wrap v) = Some v }.
+(* Definition WrapComp_W {av} (cmp: Comp W) := *)
+(*   fun (a: Value av) => match a with *)
+(*                     | SCA a => cmp ↝ a *)
+(*                     | _ => False *)
+(*                     end. *)
 
-Definition WrapComp_W {av} (cmp: Comp W) :=
-  fun (a: Value av) => match a with
-                    | SCA a => cmp ↝ a
-                    | _ => False
-                    end.
+(* Definition WrapCons_W {av} key (cmp: W -> Comp W) tail : (. *)
+  
+(*   fun (a: Value av) => match a with *)
+(*                     | SCA a => Cons key (cmp a) tail *)
+(*                     | _ => Nil *)
+(*                     end. *)
 
-Definition WrapCons_W {av} key (cmp: W -> Comp (Value av)) tail :=
-  fun (a: Value av) => match a with
-                    | SCA a => Cons key (cmp a) tail
-                    | _ => Nil
-                    end.
+(* Definition WrapComp_Generic `{FacadeWrapper (Value av) A} (cmp: Comp A) := *)
+(*   fun (a: Value av) => match (unwrap a) with *)
+(*                     | Some a => cmp ↝ a *)
+(*                     | None => False *)
+(*                     end. *)
 
-Definition WrapComp_Generic `{FacadeWrapper (Value av) A} (cmp: Comp A) :=
-  fun (a: Value av) => match (unwrap a) with
-                    | Some a => cmp ↝ a
-                    | None => False
-                    end.
+(* Definition WrapCons_Generic `{FacadeWrapper (Value av) A} key (cmp: A -> Comp (Value av)) tail := *)
+(*   fun (a: Value av) => match (unwrap a) with *)
+(*                     | Some a => Cons key (cmp a) tail *)
+(*                     | _ => Nil *)
+(*                     end. *)
 
-Definition WrapCons_Generic `{FacadeWrapper (Value av) A} key (cmp: A -> Comp (Value av)) tail :=
-  fun (a: Value av) => match (unwrap a) with
-                    | Some a => Cons key (cmp a) tail
-                    | _ => Nil
-                    end.
-
-Definition WrappedCons {av A} Wrapper (key: option string) (cmp: A -> Comp (Value av)) (tail: Value av -> Telescope av)
-  : Value av -> Telescope av :=
-  Wrapper key cmp tail.
+(* Definition WrappedCons {av A} Wrapper (key: option string) (cmp: A -> Comp (Value av)) (tail: Value av -> Telescope av) *)
+(*   : Value av -> Telescope av := *)
+(*   Wrapper key cmp tail. *)
 
 Definition AlwaysComputesToSCA {av} (v: Comp (Value av)) :=
   forall vv, v ↝ vv -> is_adt vv = false.
-
-Instance FacadeWrapper_SCA {av} : FacadeWrapper (Value av) W :=
-  {| wrap := SCA av;
-     unwrap := fun a => match a with SCA a => Some a | _ => None end;
-     wrap_unwrap := fun v => eq_refl |}.
