src/CertifiedExtraction/ComputesToLemmas.v
@@ -12,56 +12,55 @@ Transparent computes_to.
 
 (* FIXME this is a special case of below, and should be removed *)
 
-Lemma computes_to_match_SCA:
-  forall (av : Type) (compA : Comp W) (v0 : W),
-    compA ↝ v0 ->
-    (fun a : Value av =>
-       match a with
-       | SCA aa => compA aa
-       | ADT _ => False
-       end) ↝ SCA av v0.
-Proof.
-  trivial.
-Qed.
+(* Lemma computes_to_match_SCA: *)
+(*   forall (av : Type) (compA : Comp W) (v0 : W), *)
+(*     compA ↝ v0 -> *)
+(*     (fun a : Value av => *)
+(*        match a with *)
+(*        | SCA aa => compA aa *)
+(*        | ADT _ => False *)
+(*        end) ↝ SCA av v0. *)
+(* Proof. *)
+(*   trivial. *)
+(* Qed. *)
 
-Hint Resolve computes_to_match_SCA : SameValues_Fiat_db.
+(* Hint Resolve computes_to_match_SCA : SameValues_Fiat_db. *)
 
-Lemma computes_to_match_SCA_inv:
-  forall av (compA : Comp W) x,
-    (fun a : Value av =>
-       match a with
-       | SCA aa => compA aa
-       | ADT _ => False
-       end) ↝ x ->
-    exists xx, x = SCA av xx /\ compA xx.
-Proof.
-  intros; destruct x; compute in H; intuition eauto.
-Qed.
+(* Lemma computes_to_match_SCA_inv: *)
+(*   forall av (compA : Comp W) x, *)
+(*     (fun a : Value av => *)
+(*        match a with *)
+(*        | SCA aa => compA aa *)
+(*        | ADT _ => False *)
+(*        end) ↝ x -> *)
+(*     exists xx, x = SCA av xx /\ compA xx. *)
+(* Proof. *)
+(*   intros; destruct x; compute in H; intuition eauto. *)
+(* Qed. *)
 
-(* </FIXME> *)
+(* (* </FIXME> *) *)
 
-Lemma computes_to_WrapComp_Generic:
-  forall `{FacadeWrapper (Value av) A} (compA : Comp A) (v0 : A) (H : compA ↝ v0),
-    WrapComp_Generic compA ↝ (wrap v0).
-Proof.
-  unfold WrapComp_Generic, computes_to; simpl; intros.
-  rewrite wrap_unwrap.
-  trivial.
-Qed.
+(* Lemma computes_to_WrapComp_Generic: *)
+(*   forall `{FacadeWrapper (Value av) A} (compA : Comp A) (v0 : A) (H : compA ↝ v0), *)
+(*     WrapComp_Generic compA ↝ (wrap v0). *)
+(* Proof. *)
+(*   unfold WrapComp_Generic, computes_to; simpl; intros. *)
+(*   rewrite unwrap_wrap. *)
+(*   trivial. *)
+(* Qed. *)
 
-Hint Resolve computes_to_WrapComp_Generic : SameValues_Fiat_db.
+(* Hint Resolve computes_to_WrapComp_Generic : SameValues_Fiat_db. *)
 
-Lemma computes_to_WrapComp_Generic_inv:
-  forall `{FacadeWrapper (Value av) A} (compA : Comp A) x,
-    WrapComp_Generic compA ↝ x ->
-    exists xx, unwrap x = Some xx /\ compA ↝ xx.
-Proof.
-  unfold WrapComp_Generic, computes_to; simpl; intros.
-  destruct (unwrap x) eqn:eq0; intuition eauto.
-Qed.
+(* Lemma computes_to_WrapComp_Generic_inv: *)
+(*   forall `{FacadeWrapper (Value av) A} (compA : Comp A) x, *)
+(*     WrapComp_Generic compA ↝ x -> *)
+(*     exists xx, unwrap x = Some xx /\ compA ↝ xx. *)
+(* Proof. *)
+(*   unfold WrapComp_Generic, computes_to; simpl; intros. *)
+(*   destruct (unwrap x) eqn:eq0; intuition eauto. *)
+(* Qed. *)
 
-Opaque computes_to.
-
+(* Opaque computes_to. *)
 
 Lemma AlwaysComputesToSCA_ret_SCA:
   forall (av : Type) (v : W), AlwaysComputesToSCA (ret (SCA av v)).
@@ -71,35 +70,35 @@ Qed.
 
 Hint Resolve AlwaysComputesToSCA_ret_SCA : SameValues_db.
 
-Lemma AlwaysComputesToSCA_WrapComp_W {av} (cmp: Comp W) :
-  AlwaysComputesToSCA (@WrapComp_W av cmp).
-Proof.
-  Transparent computes_to.
-  red; unfold WrapComp_W, computes_to; intros.
-  destruct vv; simpl; (reflexivity || (exfalso; assumption)).
-Qed.
+(* Lemma AlwaysComputesToSCA_WrapComp_W {av} (cmp: Comp W) : *)
+(*   AlwaysComputesToSCA (@WrapComp_W av cmp). *)
+(* Proof. *)
+(*   Transparent computes_to. *)
+(*   red; unfold WrapComp_W, computes_to; intros. *)
+(*   destruct vv; simpl; (reflexivity || (exfalso; assumption)). *)
+(* Qed. *)
 
-Lemma WrapComp_W_computes_to {av} {cmp: Comp W} {v: Value av} :
-  WrapComp_W cmp ↝ v ->
-  { v' | cmp ↝ v' /\ v = SCA _ v' }.
-Proof.
-  intros; destruct v.
-  - exists w; intuition congruence.
-  - exfalso; assumption.
-Qed.
+(* Lemma WrapComp_W_computes_to {av} {cmp: Comp W} {v: Value av} : *)
+(*   WrapComp_W cmp ↝ v -> *)
+(*   { v' | cmp ↝ v' /\ v = SCA _ v' }. *)
+(* Proof. *)
+(*   intros; destruct v. *)
+(*   - exists w; intuition congruence. *)
+(*   - exfalso; assumption. *)
+(* Qed. *)
 
-Lemma WrapComp_W_rewrite:
-  forall (av : Type) (w : Word.word 32),
-    Monad.equiv (WrapComp_W (ret w)) (ret (SCA av w)).
-Proof.
-  unfold WrapComp_W; unfold Monad.equiv. (* SameValues_Fiat_t; *)
-  repeat match goal with
-         | _ => progress subst
-         | _ => progress split
-         | _ => progress intros
-         | _ => progress computes_to_inv
-         | [ H: exists x, _ |- _ ] => destruct H
-         | [ H: _ /\ _ |- _ ] => destruct H
-         | [ H: _ |- _ ] => apply computes_to_match_SCA_inv in H
-         end.
-Qed.
+(* Lemma WrapComp_W_rewrite: *)
+(*   forall (av : Type) (w : Word.word 32), *)
+(*     Monad.equiv (WrapComp_W (ret w)) (ret (SCA av w)). *)
+(* Proof. *)
+(*   unfold WrapComp_W; unfold Monad.equiv. (* SameValues_Fiat_t; *) *)
+(*   repeat match goal with *)
+(*          | _ => progress subst *)
+(*          | _ => progress split *)
+(*          | _ => progress intros *)
+(*          | _ => progress computes_to_inv *)
+(*          | [ H: exists x, _ |- _ ] => destruct H *)
+(*          | [ H: _ /\ _ |- _ ] => destruct H *)
+(*          | [ H: _ |- _ ] => apply computes_to_match_SCA_inv in H *)
+(*          end. *)
+(* Qed. *)
