src/CertifiedExtraction/Extraction.v
@@ -1,2 +1,0 @@
-Require Export CertifiedExtraction.Extraction.Binops.
-
