src/CertifiedExtraction/Extraction/BasicTactics.v
@@ -24,3 +24,9 @@ Ltac clean_DropName_in_ProgOk :=
   match_ProgOk ltac:(fun prog pre post ext env =>
                        try (is_dirty_telescope pre; clean_telescope pre ext);
                        try (is_dirty_telescope post; clean_telescope post ext)).
+
+Ltac hoare :=
+  match goal with
+  | _ => progress intros
+  | [  |- {{ _ }} (Seq _ _) {{ _ }} ∪ {{ _ }} // _ ] => eapply CompileSeq; try eassumption
+  end.
