src/CertifiedExtraction/Extraction/Basics.v
@@ -3,25 +3,25 @@ Require Import
         CertifiedExtraction.ExtendedLemmas.
 
 Lemma CompileConstant:
-  forall {av} name env w ext tenv,
+  forall {av} name env w ext (tenv: Telescope av),
     name ∉ ext ->
     NotInTelescope name tenv ->
     {{ tenv }}
       (Assign name (Const w))
-    {{ [[name <-- (SCA av w) as _]]::tenv }} ∪ {{ ext }} // env.
+    {{ [[name <-- w as _]]::tenv }} ∪ {{ ext }} // env.
 Proof.
   SameValues_Facade_t.
 Qed.
 
 Lemma CompileRead:
-  forall {av} name var (val: W) ext tenv,
+  forall {av} name var (val: W) ext (tenv: Telescope av),
     name ∉ ext ->
     NotInTelescope name tenv ->
-    StringMap.MapsTo var (SCA av val) ext ->
+    StringMap.MapsTo var (wrap val) ext ->
     forall env,
     {{ tenv }}
       (Assign name (Var var))
-    {{ [[name <-- (SCA _ val) as _]]::tenv }} ∪ {{ ext }} // env.
+    {{ [[name <-- val as _]]::tenv }} ∪ {{ ext }} // env.
 Proof.
   SameValues_Facade_t.
 Qed.
@@ -36,7 +36,7 @@ Proof.
 Qed.
 
 Lemma ProgOk_Transitivity_Cons :
-  forall {av} env ext t1 t2 prog1 prog2 k (v: Comp (Value av)),
+  forall `{FacadeWrapper (Value av) A} env ext t1 t2 prog1 prog2 k (v: Comp A),
     {{ t1 }}                     prog1      {{ [[k <~~ v as _]]::t1 }}     ∪ {{ ext }} // env ->
     {{ [[k <~~ v as _]]::t1 }}      prog2      {{ [[k <~~ v as kk]]::t2 kk }} ∪ {{ ext }} // env ->
     {{ t1 }}                Seq prog1 prog2 {{ [[k <~~ v as kk]]::t2 kk }} ∪ {{ ext }} // env.
@@ -45,7 +45,7 @@ Proof.
 Qed.
 
 Lemma ProgOk_Transitivity_Name :
-  forall {av} k env ext t1 t2 prog1 prog2 (v: Comp (Value av)),
+  forall `{FacadeWrapper (Value av) A} k env ext t1 t2 prog1 prog2 (v: Comp A),
     {{ t1 }}                          prog1        {{ [[`k <~~ v as kk]]::t2 kk }} ∪ {{ ext }} // env ->
     {{ [[`k <~~ v as kk]]::t2 kk }}      prog2        {{ [[v as kk]]::t2 kk }} ∪ {{ ext }} // env ->
     {{ t1 }}                      Seq prog1 prog2  {{ [[v as kk]]::t2 kk }} ∪ {{ ext }} // env.
@@ -54,7 +54,7 @@ Proof.
 Qed.
 
 Lemma ProgOk_Transitivity_Name' :
-  forall {av} k env ext t1 t2 prog1 prog2 (v: Comp (Value av)),
+  forall `{FacadeWrapper (Value av) A} k env ext t1 t2 prog1 prog2 (v: Comp A),
     {{ t1 }}                     prog1        {{ [[`k <~~ v as _]]::t1 }} ∪ {{ ext }} // env ->
     {{ [[`k <~~ v as _]]::t1 }}     prog2        {{ [[v as kk]]::t2 kk }} ∪ {{ ext }} // env ->
     {{ t1 }}                 Seq prog1 prog2  {{ [[v as kk]]::t2 kk }} ∪ {{ ext }} // env.
