src/CertifiedExtraction/Extraction/Conditionals.v
@@ -4,44 +4,44 @@ Require Import
 
 Lemma isTrueExpr_is_true:
   forall {av} (tmp : string) (st' : State av),
-    StringMap.MapsTo tmp (bool2val true) st' -> is_true st' (isTrueExpr tmp).
+    StringMap.MapsTo tmp (wrap (bool2w true)) st' -> is_true st' (isTrueExpr tmp).
 Proof.
-  unfold isTrueExpr, bool2val, is_true, is_false, eval_bool; simpl;
+  unfold isTrueExpr, is_true, is_false, eval_bool; simpl;
   SameValues_Facade_t.
 Qed.
 
 Lemma isTrueExpr_is_false:
   forall {av} (tmp : string) (st' : State av),
-    StringMap.MapsTo tmp (bool2val false) st' -> is_false st' (isTrueExpr tmp).
+    StringMap.MapsTo tmp (wrap (bool2w false)) st' -> is_false st' (isTrueExpr tmp).
 Proof.
-  unfold isTrueExpr, bool2val, is_true, is_false, eval_bool; simpl;
+  unfold isTrueExpr, is_true, is_false, eval_bool; simpl;
   SameValues_Facade_t.
 Qed.
 
 Lemma is_true_isTrueExpr:
-  forall {av} (gallinaTest : bool) (tmp : StringMap.key) (st' : State av),
+  forall {av} {gallinaTest : bool} {tmp : StringMap.key} (st' : State av),
     is_true st' (isTrueExpr tmp) ->
-    StringMap.MapsTo tmp (bool2val gallinaTest) st' ->
+    StringMap.MapsTo tmp (wrap (bool2w gallinaTest)) st' ->
     gallinaTest = true.
 Proof.
-  unfold isTrueExpr, bool2val, bool2w, is_true, is_false, eval_bool; simpl;
+  unfold isTrueExpr, bool2w, is_true, is_false, eval_bool; simpl;
   destruct gallinaTest; SameValues_Facade_t.
 Qed.
 
 Lemma is_false_isTrueExpr:
-  forall {av} (gallinaTest : bool) (tmp : StringMap.key) (st' : State av),
+  forall {av} {gallinaTest : bool} {tmp : StringMap.key} (st' : State av),
     is_false st' (isTrueExpr tmp) ->
-    StringMap.MapsTo tmp (bool2val gallinaTest) st' ->
+    StringMap.MapsTo tmp (wrap (bool2w gallinaTest)) st' ->
     gallinaTest = false.
 Proof.
-  unfold isTrueExpr, bool2val, bool2w, is_true, is_false, eval_bool; simpl;
+  unfold isTrueExpr, bool2w, is_true, is_false, eval_bool; simpl;
   destruct gallinaTest; SameValues_Facade_t.
 Qed.
 
 Ltac facade_if_helper :=
   match goal with
-  | [ H: is_true ?st (isTrueExpr ?k), H': StringMap.MapsTo ?k (bool2val ?test) ?st |- _ ] => learn (is_true_isTrueExpr H H')
-  | [ H: is_false ?st (isTrueExpr ?k), H': StringMap.MapsTo ?k (bool2val ?test) ?st |- _ ] => learn (is_false_isTrueExpr H H')
+  | [ H: is_true ?st (isTrueExpr ?k), H': StringMap.MapsTo ?k (wrap (bool2w ?test)) ?st |- _ ] => learn (is_true_isTrueExpr H H')
+  | [ H: is_false ?st (isTrueExpr ?k), H': StringMap.MapsTo ?k (wrap (bool2w ?test)) ?st |- _ ] => learn (is_false_isTrueExpr H H')
   | _ => solve [eauto using isTrueExpr_is_false, isTrueExpr_is_true with SameValues_db]
   end.
 
@@ -51,18 +51,21 @@ Lemma CompileIf :
     NotInTelescope tmp tenv ->
     {{ tenv }}
       facadeTest
-    {{ [[tmp <-- (bool2val gallinaTest) as _]]::tenv }} ∪ {{ ext }} // env ->
-    {{ [[tmp <-- (bool2val gallinaTest) as _]]::tenv }}
+    {{ [[tmp <-- (bool2w gallinaTest) as _]]::tenv }} ∪ {{ ext }} // env ->
+    {{ [[tmp <-- (bool2w gallinaTest) as _]]::tenv }}
       facadeT
-    {{ [[tmp <-- (bool2val gallinaTest) as _]]::[[`k <~~ gallinaT as _]]::tenv }} ∪ {{ ext }} // env ->
-    {{ [[tmp <-- (bool2val gallinaTest) as _]]::tenv }}
+    {{ [[tmp <-- (bool2w gallinaTest) as _]]::[[`k <~~ gallinaT as _]]::tenv }} ∪ {{ ext }} // env ->
+    {{ [[tmp <-- (bool2w gallinaTest) as _]]::tenv }}
       facadeF
-    {{ [[tmp <-- (bool2val gallinaTest) as _]]::[[`k <~~ gallinaF as _]]::tenv }} ∪ {{ ext }} // env ->
+    {{ [[tmp <-- (bool2w gallinaTest) as _]]::[[`k <~~ gallinaF as _]]::tenv }} ∪ {{ ext }} // env ->
     {{ tenv }}
       (Seq facadeTest (If (isTrueExpr tmp) facadeT facadeF))
     {{ [[`k <~~ if gallinaTest then gallinaT else gallinaF as _]]::tenv }} ∪ {{ ext }} // env.
 Proof.
-  repeat (SameValues_Facade_t_step || facade_if_helper).
+  repeat match goal with
+         | _ => SameValues_Facade_t_step
+         | _ => facade_if_helper
+         end.
 Qed.
 
 Lemma CompileIf_InPlace :
@@ -71,13 +74,13 @@ Lemma CompileIf_InPlace :
     NotInTelescope tmp tenv ->
     {{ [[`k <~~ oldK as kk]] :: tenv }}
       facadeTest
-    {{ [[tmp <-- (bool2val gallinaTest) as _]]::[[`k <~~ oldK as _]] :: tenv }} ∪ {{ ext }} // env ->
-    {{ [[tmp <-- (bool2val gallinaTest) as _]]::[[`k <~~ oldK as _]] :: tenv }}
+    {{ [[tmp <-- (bool2w gallinaTest) as _]]::[[`k <~~ oldK as _]] :: tenv }} ∪ {{ ext }} // env ->
+    {{ [[tmp <-- (bool2w gallinaTest) as _]]::[[`k <~~ oldK as _]] :: tenv }}
       facadeT
-    {{ [[tmp <-- (bool2val gallinaTest) as _]]::[[`k <~~ gallinaT as _]]::tenv }} ∪ {{ ext }} // env ->
-    {{ [[tmp <-- (bool2val gallinaTest) as _]]::[[`k <~~ oldK as _]] :: tenv }}
+    {{ [[tmp <-- (bool2w gallinaTest) as _]]::[[`k <~~ gallinaT as _]]::tenv }} ∪ {{ ext }} // env ->
+    {{ [[tmp <-- (bool2w gallinaTest) as _]]::[[`k <~~ oldK as _]] :: tenv }}
       facadeF
-    {{ [[tmp <-- (bool2val gallinaTest) as _]]::[[`k <~~ gallinaF as _]]::tenv }} ∪ {{ ext }} // env ->
+    {{ [[tmp <-- (bool2w gallinaTest) as _]]::[[`k <~~ gallinaF as _]]::tenv }} ∪ {{ ext }} // env ->
     {{ [[`k <~~ oldK as _]] :: tenv }}
       (Seq facadeTest (DFacade.If (isTrueExpr tmp) facadeT facadeF))
     {{ [[`k <~~ if gallinaTest then gallinaT else gallinaF as _]]::tenv }} ∪ {{ ext }} // env.
