src/CertifiedExtraction/Extraction/DeallocSCA.v
@@ -2,8 +2,7 @@ Require Import
         CertifiedExtraction.Extraction.Core.
 
 Lemma CompileDeallocSCA:
-  forall {av} (env : Env av) k compSCA tail tail' ext prog,
-    AlwaysComputesToSCA compSCA ->
+  forall {av} (env : Env av) k (compSCA: Comp W) tail tail' ext prog,
     {{ [[compSCA as kk]]::(tail kk)}}
       prog
     {{ [[compSCA as kk]]::(tail' kk) }} ∪ {{ ext }} // env ->
@@ -12,30 +11,30 @@ Lemma CompileDeallocSCA:
     {{ [[compSCA as kk]]::(tail' kk) }} ∪ {{ ext }} // env.
 Proof.
   SameValues_Facade_t;
-  apply SameValues_Dealloc_SCA in H1;
+  apply SameValues_Dealloc_SCA in H0;
   SameValues_Facade_t.
 Qed.
 
 Lemma CompileDeallocSCA_ret:
   forall {av} (env : Env av) k v tail tail' ext
     prog,
-    {{ [[(ret (SCA _ v)) as kk]]::(tail kk)}}
+    {{ [[(ret v) as kk]]::(tail kk)}}
       prog
-    {{ [[(ret (SCA _ v)) as kk]]::(tail' kk) }} ∪ {{ ext }} // env ->
-    {{ [[k <~~ ret (SCA _ v) as kk]]::(tail kk)}}
+    {{ [[(ret v) as kk]]::(tail' kk) }} ∪ {{ ext }} // env ->
+    {{ [[k <~~ ret v as kk]]::(tail kk)}}
       prog
-    {{ [[ret (SCA _ v) as kk]]::(tail' kk) }} ∪ {{ ext }} // env.
+    {{ [[ret v as kk]]::(tail' kk) }} ∪ {{ ext }} // env.
 Proof.
   intros; apply CompileDeallocSCA;
   SameValues_Facade_t.
 Qed.
 
 Lemma CompileDeallocSCA_discretely :
-  forall {av} tenv tenv' ext env k v prog,
+  forall {av} (tenv tenv': Telescope av) ext env k v prog,
     k ∉ ext ->
     NotInTelescope k tenv ->
-    {{ [[k <-- SCA av v as _]] :: tenv }} prog {{ [[k <-- SCA av v as _]] :: tenv' }} ∪ {{ ext }} // env ->
-    {{ [[k <-- SCA av v as _]] :: tenv }} prog {{ tenv' }} ∪ {{ ext }} // env.
+    {{ [[k <-- v as _]] :: tenv }} prog {{ [[k <-- v as _]] :: tenv' }} ∪ {{ ext }} // env ->
+    {{ [[k <-- v as _]] :: tenv }} prog {{ tenv' }} ∪ {{ ext }} // env.
 Proof.
   SameValues_Facade_t.
 Qed.
