src/CertifiedExtraction/Extraction/DeallocSCATactics.v
@@ -4,10 +4,7 @@ Require Import
 
 Ltac compile_dealloc key cmp :=
   debug "Deallocating head binding" key;
-  match cmp with
-  | _ => apply CompileDeallocSCA; [ solve [eauto with dealloc_db] | ]
-  | ret (@ADT _ ?x) => fail
-  end.
+  apply CompileDeallocSCA.
 
-Hint Resolve AlwaysComputesToSCA_ret_SCA : dealloc_db.
-Hint Resolve AlwaysComputesToSCA_WrapComp_W : dealloc_db.
+Hint Resolve AlwaysComputesToSCA_ret_SCA : dealloc_db. (* FIXME remove *)
+
