src/CertifiedExtraction/Extraction/External/GenericMethods.v
@@ -4,7 +4,7 @@ Require Import
 
 Definition FacadeImplementationWW av (fWW: W -> W) : AxiomaticSpec av.
   refine {|
-      PreCond := fun args => exists x, args = (SCA av x) :: nil;
-      PostCond := fun args ret => exists x, args = (SCA av x, None) :: nil /\ ret = SCA av (fWW x)
+      PreCond := fun args => exists x, args = (wrap x) :: nil;
+      PostCond := fun args ret => exists x, args = (wrap x, None) :: nil /\ ret = wrap (fWW x)
     |}; spec_t.
 Defined.
