src/CertifiedExtraction/Utils.v
@@ -5,11 +5,25 @@ Require Export
         CertifiedExtraction.PureUtils
         CertifiedExtraction.FacadeUtils.
 
+Lemma wrap_inj `{FacadeWrapper AA A} :
+  forall (a1 a2: A),
+    wrap a1 = wrap a2 -> a1 = a2.
+Proof.
+  intros.
+  cut (Some a1 = Some a2); [ congruence | ].
+  rewrite <- !unwrap_wrap.
+  congruence.
+Qed.
+
 Ltac cleanup :=
   match goal with
   | _ => cleanup_pure
   | _ => cleanup_facade_pure
   | _ => progress computes_to_inv
+  | [ H: wrap _ = wrap _ |- _ ] => apply wrap_inj in H
+  | [ H: unwrap ?v = Some ?vv |- _ ] => apply wrap_unwrap in H; subst v
+  | [  |- context[unwrap (wrap _)] ] => rewrite unwrap_wrap
+  | [ H: context[unwrap (wrap _)] |- _ ] => rewrite unwrap_wrap in H
   end.
 
 Ltac wipe :=
